PRF goal

proof/SomeDKC.ec
@@ -1,6 +1,10 @@
 require import Int.
 require import Bool.
+require import Real.
+require import NewFMap.
+require import FSet.
 require ConcretePRF.
+require IdealPRF.
 
 require (*--*) DKC.
 require (*--*) DKCSec2.
@@ -19,6 +23,11 @@ theory SomeDKC.
 	type D = word,
 	type R = word.
 
+  clone import IdealPRF with
+	type K = KW.word,
+	type D = word,
+	type R = word.
+        
   op E(t,k1,k2,m) = (F k1 t) ^ (F k2 t) ^ m.
   op D(t,k1,k2,c) = (F k1 t) ^ (F k2 t) ^ c.
 
@@ -49,3 +58,67 @@ theory SomeDKC.
       game; otherwise, we are in a OTP world, because tweaks do not
       repeat. *)  
 
+section SomeDKC_Proof.
+  
+declare module A : Adv_DKC_t.
+
+op bound: int.
+
+module Dp = {
+    var kpub : ((int * bool), word) fmap
+    var used : word fset
+  }.
+
+module D(F:PRF_Oracle) = {
+  proc distinguish(lsb : bool,l : int): bool= {
+      var i : int;
+    
+      i = 0;
+      while (i < bound) {
+        DKCp.kpub.[(i, false)] = WD.zeros;
+        DKCp.kpub.[(i, true)] = WD.zeros;
+        i = i + 1;
+      }
+            
+      i = 0;
+      while (i < bound) {
+        if (i = DKCp.l) {
+          DKCp.lsb = ${0,1};
+          DKCp.ksec = $Dword.dwordLsb (DKCp.lsb);
+          (* DKCp.kpub.[(i,DKCp.lsb)] = witness;  can never return or encrypt this key *)
+          DKCp.kpub.[(i,!DKCp.lsb)] = $Dword.dwordLsb (!DKCp.lsb);  
+        }
+        else {
+          tok1 = $Dword.dwordLsb (false);
+          tok2 = $Dword.dwordLsb (true);
+            DKCp.kpub.[(i, false)] = tok1;
+            DKCp.kpub.[(i, true)] = tok2;
+        }
+        i = i + 1;
+      }
+     
+      return DKCp.lsb;
+    }
+   
+}.
+
+equiv true_key : 
+    DKCSecurity.Game(DKC, A).game ~
+    IND(PRFr_Wrapped,D).main : 0 <= l{1} && b{1} = true
+                               ==> ={res}.
+    proof.
+      proc. inline DKC.initialize PRFr_Wrapped.init D(PRFr_Wrapped).distinguish.
+
+
+    
+lemma PrfDKC_secure : forall &m i, 0 <= i =>
+    Pr[DKCSecurity.Game(DKC, A).game(true,i)@ &m:res] - 
+    Pr[DKCSecurity.Game(DKC, A).game(false,i)@ &m:!res] =
+    Pr[IND(PRFr_Wrapped,D).main()@ &m:res] - Pr[IND(RandomFunction,D).main()@ &m:!res].
+    move => &m i  H.
+    admit.
+  qed.
+
+  end section SomeDKC_Proof.
+  
+end SomeDKC.
